translator/ml_optimiseScript.sml
@@ -3,7 +3,7 @@ val _ = new_theory "ml_optimise";
 local open intLib in end;
 open astTheory libTheory semanticPrimitivesTheory bigStepTheory;
 open terminationTheory;
-open bigClockTheory;
+open bigClockTheory determTheory;
 open arithmeticTheory listTheory combinTheory pairTheory;
 open integerTheory ml_translatorTheory;
 
@@ -148,7 +148,7 @@ val BOTTOM_UP_OPT_THM = prove(
 
 val abs2let_def = Define `
   abs2let x =
-     case x of (App Opapp (Fun v exp) y) => Let v y exp
+     case x of (App Opapp (Fun v exp) y) => Let (SOME v) y exp
              | rest => rest`;
 
 val abs2let_thm = prove(
@@ -163,14 +163,14 @@ val abs2let_thm = prove(
   \\ Q.LIST_EXISTS_TAC [`v2`,`count',s3`] \\ FULL_SIMP_TAC std_ss []
   \\ Q.PAT_ASSUM `evaluate F env s (Fun s' e') ((s2,Rval v1))` MP_TAC
   \\ SIMP_TAC (srw_ss()) [Once evaluate_cases,do_app_def]
-  \\ REPEAT STRIP_TAC \\ FULL_SIMP_TAC (srw_ss()) []);
+  \\ REPEAT STRIP_TAC \\ FULL_SIMP_TAC (srw_ss()) [opt_bind_def,bind_def]);
 
 
 (* rewrite optimisation: let x = y in x --> y *)
 
 val let_id_def = Define `
-  (let_id (Let v x y) =
-     if (y = Var (Short v)) then x else Let v x y) /\
+  (let_id (Let (SOME v) x y) =
+     if (y = Var (Short v)) then x else Let (SOME v) x y) /\
   (let_id rest = rest)`;
 
 val let_id_thm = prove(
@@ -181,7 +181,8 @@ val let_id_thm = prove(
   \\ SIMP_TAC (srw_ss()) [Once evaluate_cases]
   \\ REPEAT STRIP_TAC \\ POP_ASSUM MP_TAC
   \\ SIMP_TAC (srw_ss()) [Once evaluate_cases,bind_def,lookup_def]
-  \\ REPEAT STRIP_TAC \\ FULL_SIMP_TAC (srw_ss()) [lookup_var_id_def]);
+  \\ REPEAT STRIP_TAC
+  \\ FULL_SIMP_TAC (srw_ss()) [lookup_var_id_def,opt_bind_def]);
 
 
 (* rewrite optimisations: x - n + n --> x and x + n - n --> x *)
@@ -212,8 +213,7 @@ val do_app_IMP = prove(
   ``(do_app s env (Opn opn) v1 v2 = SOME (s1,env1,e3)) ==>
     ?i1 i2. (v1 = Litv (IntLit i1)) /\ (v2 = Litv (IntLit i2))``,
   FULL_SIMP_TAC (srw_ss()) [do_app_def]
-  \\ REPEAT (BasicProvers.FULL_CASE_TAC)
-  \\ FULL_SIMP_TAC (srw_ss()) []);
+  \\ REPEAT (BasicProvers.FULL_CASE_TAC));
 
 val evaluate_11_Rval = prove(
   ``evaluate ck env s exp (t,Rval res1) ==>
@@ -254,469 +254,11 @@ val opt_sub_add_thm = prove(
        intLib.COOPER_PROVE ``i + i2 - i2 = i:int``,
        intLib.COOPER_PROVE ``i - i2 + i2 = i:int``]);
 
-(*
-
-(* integer "if-decide" optimisation *)
-
-val pat_size_lemma = prove(
-  ``!xs a. MEM a xs ==> pat_size a < pat1_size xs``,
-  Induct \\ FULL_SIMP_TAC (srw_ss()) [pat_size_def]
-  \\ REPEAT STRIP_TAC \\ FULL_SIMP_TAC std_ss [] \\ RES_TAC \\ DECIDE_TAC);
-
-val pat_vars_def = tDefine "pat_vars" `
-  (pat_vars (Pvar v _) = [v]) /\
-  (pat_vars (Pref p) = pat_vars p) /\
-  (pat_vars (Plit _) = []) /\
-  (pat_vars (Pcon c xs) = FLAT (MAP pat_vars xs))`
- (WF_REL_TAC `measure (pat_size)` THEN REPEAT STRIP_TAC
-  THEN IMP_RES_TAC pat_size_lemma THEN DECIDE_TAC);
-
-val _ = Hol_datatype `
-  int_cmp = IntUnkown | IntLessEq of int => string
-                      | IntGreater of int => string`;
-
-val get_fact_def = Define `
-  (get_fact (App (Opb Gt) (Var v NONE) ((Lit (IntLit i)))) = IntLessEq (i+1) v) /\
-  (get_fact (App (Opb Geq) (Var v NONE) ((Lit (IntLit i)))) = IntLessEq i v) /\
-  (get_fact (App (Opb Lt) ((Lit (IntLit i))) (Var v NONE)) = IntLessEq (i+1) v) /\
-  (get_fact (App (Opb Leq) ((Lit (IntLit i))) (Var v NONE)) = IntLessEq i v) /\
-  (get_fact (App (Opb Gt) ((Lit (IntLit i))) (Var v NONE)) = IntGreater i v) /\
-  (get_fact (App (Opb Geq) ((Lit (IntLit i))) (Var v NONE)) = IntGreater (i+1) v) /\
-  (get_fact (App (Opb Lt) (Var v NONE) ((Lit (IntLit i)))) = IntGreater i v) /\
-  (get_fact (App (Opb Leq) (Var v NONE) ((Lit (IntLit i)))) = IntGreater (i+1) v) /\
-  (get_fact _ = IntUnkown)`;
-
-val int_negate_def = Define `
-  (int_negate IntUnkown = IntUnkown) /\
-  (int_negate (IntLessEq i v) = IntGreater i v) /\
-  (int_negate (IntGreater i v) = IntLessEq i v)`;
-
-val add_pos_fact_def = Define `add_pos_fact x b = get_fact x :: b`;
-val add_neg_fact_def = Define `add_neg_fact x b = int_negate (get_fact x) :: b`;
-
-val decide_guard_def = Define `
-  (decide_guard (IntLessEq i v) (IntLessEq j w::xs) =
-     if (v = w) /\ i <= j then SOME T else
-       decide_guard (IntLessEq i v) xs) /\
-  (decide_guard (IntLessEq i v) (IntGreater j w::xs) =
-     if (v = w) /\ j <= i then SOME F else
-       decide_guard (IntLessEq i v) xs) /\
-  (decide_guard (IntGreater i v) (IntGreater j w::xs) =
-     if (v = w) /\ j <= i then SOME T else
-       decide_guard (IntGreater i v) xs) /\
-  (decide_guard (IntGreater i v) (IntLessEq j w::xs) =
-     if (v = w) /\ i <= j then SOME F else
-       decide_guard (IntGreater i v) xs) /\
-  (decide_guard _ [] = NONE) /\
-  (decide_guard g (x::xs) = decide_guard g xs)`
-
-val int_cmp_sem_def = Define `
-  (int_cmp_sem (env:envE) res IntUnkown = T) /\
-  (int_cmp_sem env res (IntLessEq i v) =
-     ?j t. (lookup v env = SOME (Litv (IntLit j),t)) /\ (i <= j = res)) /\
-  (int_cmp_sem env res (IntGreater i v) =
-     ?j t. (lookup v env = SOME (Litv (IntLit j),t)) /\ (j < i = res))`;
-
-val case_LEMMA = prove(
-  ``!t. (case t of NONE => v | SOME (y,z) => v) = v``,
-  Cases \\ SIMP_TAC (srw_ss()) [] \\ Cases_on `x` \\ SIMP_TAC (srw_ss()) []);
-
-val get_fact_thm_T = prove(
-  ``!x env.
-      evaluate' s env x (s1,Rval (Litv (Bool T))) ==>
-      int_cmp_sem env T ((get_fact x))``,
-  HO_MATCH_MP_TAC (fetch "-" "get_fact_ind")
-  \\ FULL_SIMP_TAC std_ss [get_fact_def,int_negate_def,int_cmp_sem_def]
-  \\ ONCE_REWRITE_TAC [evaluate'_cases] \\ FULL_SIMP_TAC (srw_ss()) []
-  \\ SIMP_TAC (srw_ss()) [do_app_def]
-  \\ REPEAT STRIP_TAC
-  \\ TRY (Cases_on `v1` \\ FULL_SIMP_TAC (srw_ss()) [])
-  \\ TRY (Cases_on `l` \\ FULL_SIMP_TAC (srw_ss()) [])
-  \\ TRY (Cases_on `v2` \\ FULL_SIMP_TAC (srw_ss()) [])
-  \\ TRY (Cases_on `l` \\ FULL_SIMP_TAC (srw_ss()) [])
-  \\ TRY (Q.PAT_ASSUM `Lit xxx = e` (fn th => FULL_SIMP_TAC std_ss [GSYM th]))
-  \\ FULL_SIMP_TAC (srw_ss()) [opb_lookup_def,evaluate_Lit]
-  \\ REPEAT (POP_ASSUM MP_TAC)
-  \\ ONCE_REWRITE_TAC [evaluate'_cases] \\ FULL_SIMP_TAC (srw_ss()) [do_tapp_def]
-  \\ REPEAT STRIP_TAC \\ FULL_SIMP_TAC std_ss [case_LEMMA]
-  \\ Q.PAT_ASSUM `Litv xx = yy` (ASSUME_TAC o GSYM)
-  \\ FULL_SIMP_TAC (srw_ss()) []
-  \\ FULL_SIMP_TAC std_ss [INT_NOT_LT,INT_NOT_LE,int_ge,int_gt]
-  \\ REPEAT (Q.PAT_ASSUM `(iii:int) > jjj` MP_TAC)
-  \\ REPEAT (Q.PAT_ASSUM `(iii:int) >= jjj` MP_TAC)
-  \\ REPEAT (Q.PAT_ASSUM `(iii:int) < jjj` MP_TAC)
-  \\ REPEAT (Q.PAT_ASSUM `(iii:int) <= jjj` MP_TAC)
-  \\ REPEAT (POP_ASSUM (K ALL_TAC))
-  \\ intLib.COOPER_TAC);
-
-val get_fact_thm_F = prove(
-  ``!x env.
-      evaluate' s env x (s1,Rval (Litv (Bool F))) ==>
-      int_cmp_sem env T (int_negate (get_fact x))``,
-  HO_MATCH_MP_TAC (fetch "-" "get_fact_ind")
-  \\ FULL_SIMP_TAC std_ss [get_fact_def,int_negate_def,int_cmp_sem_def]
-  \\ ONCE_REWRITE_TAC [evaluate'_cases] \\ FULL_SIMP_TAC (srw_ss()) []
-  \\ SIMP_TAC (srw_ss()) [do_app_def]
-  \\ REPEAT STRIP_TAC
-  \\ TRY (Cases_on `v1` \\ FULL_SIMP_TAC (srw_ss()) [])
-  \\ TRY (Cases_on `l` \\ FULL_SIMP_TAC (srw_ss()) [])
-  \\ TRY (Cases_on `v2` \\ FULL_SIMP_TAC (srw_ss()) [])
-  \\ TRY (Cases_on `l` \\ FULL_SIMP_TAC (srw_ss()) [])
-  \\ TRY (Q.PAT_ASSUM `Lit xxx = e` (fn th => FULL_SIMP_TAC std_ss [GSYM th]))
-  \\ FULL_SIMP_TAC (srw_ss()) [opb_lookup_def,evaluate_Lit]
-  \\ REPEAT (POP_ASSUM MP_TAC)
-  \\ ONCE_REWRITE_TAC [evaluate'_cases] \\ FULL_SIMP_TAC (srw_ss()) [do_tapp_def]
-  \\ REPEAT STRIP_TAC \\ FULL_SIMP_TAC std_ss [case_LEMMA]
-  \\ Q.PAT_ASSUM `Litv xx = yy` (ASSUME_TAC o GSYM)
-  \\ FULL_SIMP_TAC (srw_ss()) []
-  \\ FULL_SIMP_TAC std_ss [INT_NOT_LT,INT_NOT_LE,int_ge,int_gt]
-  \\ REPEAT (Q.PAT_ASSUM `(iii:int) > jjj` MP_TAC)
-  \\ REPEAT (Q.PAT_ASSUM `(iii:int) >= jjj` MP_TAC)
-  \\ REPEAT (Q.PAT_ASSUM `(iii:int) < jjj` MP_TAC)
-  \\ REPEAT (Q.PAT_ASSUM `(iii:int) <= jjj` MP_TAC)
-  \\ REPEAT (POP_ASSUM (K ALL_TAC))
-  \\ intLib.COOPER_TAC);
-
-val decide_guard_thm = prove(
-  ``!env b x.
-      EVERY (int_cmp_sem env T) b ==>
-      !res. (decide_guard x b = SOME res) ==> int_cmp_sem env res x``,
-  STRIP_TAC \\ Induct \\ Cases_on `x` \\ SIMP_TAC std_ss [decide_guard_def]
-  \\ Cases \\ FULL_SIMP_TAC std_ss [decide_guard_def,EVERY_DEF]
-  \\ Cases_on `s' = s` \\ FULL_SIMP_TAC std_ss [decide_guard_def,EVERY_DEF]
-  \\ SRW_TAC [] [] \\ FULL_SIMP_TAC (srw_ss()) [int_cmp_sem_def]
-  \\ intLib.COOPER_TAC);
-
-val int_cmp_keep_def = Define `
-  (int_cmp_keep vs IntUnkown = F) /\
-  (int_cmp_keep vs (IntLessEq i v) = ~MEM v vs) /\
-  (int_cmp_keep vs (IntGreater i v) = ~MEM v vs)`;
-
-val int_read_exp_def = Define `
-  (int_read_exp (Var v _) = SOME (v,0)) /\
-  (int_read_exp (App (Opn Plus) (Var v _) ((Lit (IntLit i)))) = SOME (v,i)) /\
-  (int_read_exp (App (Opn Minus) (Var v _) ((Lit (IntLit i)))) = SOME (v,0-i)) /\
-  (int_read_exp _ = NONE)`;
-
-val int_cmp_apply_def = Define `
-  (int_cmp_apply (name,v,i) [] = []) /\
-  (int_cmp_apply (name,v,i) (IntUnkown::xs) = int_cmp_apply (name,v,i) xs) /\
-  (int_cmp_apply (name,v,i) ((IntLessEq (j:int) w)::xs) =
-     if v = w then IntLessEq (j+i) name :: int_cmp_apply (name,v,i) xs
-              else int_cmp_apply (name,v,i) xs) /\
-  (int_cmp_apply (name,v,i) ((IntGreater j w)::xs) =
-     if v = w then IntGreater (j+i) name :: int_cmp_apply (name,v,i) xs
-              else int_cmp_apply (name,v,i) xs)`;
-
-val int_cmp_let_def = Define `
-  int_cmp_let name x b =
-    case int_read_exp x of
-      NONE => []
-    | (SOME (v,i)) => int_cmp_apply (name,v,i) b`;
-
-val INT_IF_OPT_def = tDefine "INT_IF_OPT" `
-  (INT_IF_OPT b (Lit v) = Lit v) /\
-  (INT_IF_OPT b (Raise ex) = Raise ex) /\
-  (INT_IF_OPT b (Var name t) = Var name t) /\
-  (INT_IF_OPT b (Con tag xs) = Con tag (MAP (INT_IF_OPT b) xs)) /\
-  (INT_IF_OPT b (Fun name tt x) = Fun name tt x) /\
-  (INT_IF_OPT b (Uapp uop x1) = Uapp uop (INT_IF_OPT b x1)) /\
-  (INT_IF_OPT b (App op x1 x2) = App op (INT_IF_OPT b x1) (INT_IF_OPT b x2)) /\
-  (INT_IF_OPT b (Log l x1 x2) = Log l (INT_IF_OPT b x1) (INT_IF_OPT b x2)) /\
-  (INT_IF_OPT b (If x1 x2 x3) =
-     case decide_guard (get_fact x1) b of
-       NONE => If (INT_IF_OPT b x1) (INT_IF_OPT (add_pos_fact x1 b) x2)
-                                    (INT_IF_OPT (add_neg_fact x1 b) x3)
-     | SOME T => (INT_IF_OPT b x2)
-     | SOME F => (INT_IF_OPT b x3)) /\
-  (INT_IF_OPT b (Mat x ys) = Mat (INT_IF_OPT b x) (MAP (\(p,x). (p,INT_IF_OPT (FILTER (int_cmp_keep (pat_vars p)) b) x)) ys)) /\
-  (INT_IF_OPT b (Let oo name tt x1 x2) = Let oo name tt (INT_IF_OPT b x1)
-     (INT_IF_OPT (int_cmp_let name x1 b ++ FILTER (int_cmp_keep [name]) b) x2)) /\
-  (INT_IF_OPT b (Letrec z1 z2) = Letrec z1 z2) /\
-  (INT_IF_OPT b other = other)`
- (WF_REL_TAC `measure (exp_size o SND)` THEN REPEAT STRIP_TAC
-  THEN IMP_RES_TAC MEM_exp_size1 THEN IMP_RES_TAC MEM_exp_size2 THEN DECIDE_TAC)
-
-val MAT_INT_IF_OPT_def = Define `
-  MAT_INT_IF_OPT b ys =
-    MAP (\(p,x'). (p,INT_IF_OPT (FILTER (int_cmp_keep (pat_vars p)) b) x')) ys`;
-
-val INT_IF_OPT_def = INT_IF_OPT_def |> REWRITE_RULE [GSYM MAT_INT_IF_OPT_def]
-
-val decide_guard_IMP = prove(
-  ``!b x res. (decide_guard x b = SOME res) ==> ~(x = IntUnkown)``,
-  Induct \\ FULL_SIMP_TAC std_ss [decide_guard_def]);
-
-val IMP_int_negate = prove(
-  ``!x. ~(x = IntUnkown) ==> ~(int_negate x = IntUnkown)``,
-  Cases \\ EVAL_TAC);
-
-val int_cmp_sem_NOT = prove(
-  ``!x env. int_cmp_sem env F x /\ int_cmp_sem env T x /\ ~(x = IntUnkown) ==> F``,
-  REPEAT STRIP_TAC \\ Cases_on `x`
-  \\ FULL_SIMP_TAC (srw_ss()) [int_cmp_sem_def]
-  \\ FULL_SIMP_TAC (srw_ss()) [int_cmp_sem_def]
-  \\ FULL_SIMP_TAC std_ss [INT_NOT_LT,INT_NOT_LE,int_ge,int_gt]
-  \\ REPEAT (Q.PAT_ASSUM `(iii:int) > jjj` MP_TAC)
-  \\ REPEAT (Q.PAT_ASSUM `(iii:int) >= jjj` MP_TAC)
-  \\ REPEAT (Q.PAT_ASSUM `(iii:int) < jjj` MP_TAC)
-  \\ REPEAT (Q.PAT_ASSUM `(iii:int) <= jjj` MP_TAC)
-  \\ FULL_SIMP_TAC std_ss []
-  \\ REPEAT (POP_ASSUM (K ALL_TAC))
-  \\ intLib.COOPER_TAC);
-
-val int_cmp_sem_negate = prove(
-  ``!x env. int_cmp_sem env T (int_negate x) ==> int_cmp_sem env F x``,
-  Cases \\ FULL_SIMP_TAC std_ss [int_cmp_sem_def,int_negate_def]
-  \\ REPEAT STRIP_TAC \\ FULL_SIMP_TAC (srw_ss()) [] \\ intLib.COOPER_TAC);
-
-val isRval_def = Define `(isRval (Rval _) = T) /\ (isRval _ = F)`;
-
-val lookup_ZIP_APPEND = prove(
-  ``!xs ys s x.
-      (LENGTH xs = LENGTH ys) /\ ~(MEM s xs) ==>
-      (lookup s (ZIP (xs,ys) ++ x) = lookup s x)``,
-  Induct \\ Cases_on `ys` \\ FULL_SIMP_TAC (srw_ss()) [LENGTH,ADD1,ZIP,lookup_def]);
-
-val IMP_IMP = METIS_PROVE [] ``b1 /\ (b3 ==> b2) ==> ((b1 ==> b3) ==> b2)``
-
-val ZIP_APPEND = prove(
-  ``!xs ys xs1 ys2.
-      (LENGTH xs = LENGTH ys) /\ (LENGTH xs1 = LENGTH ys1) ==>
-      (ZIP (xs,ys) ++ ZIP (xs1,ys1) = ZIP (xs++xs1, ys++ys1))``,
-  Induct \\ Cases_on `ys` \\ FULL_SIMP_TAC (srw_ss()) []);
-
-val pmatch_lemma = prove(
-   ``!p x2 env env1.
-       (pmatch' s p x2 env = Match env1) ==>
-       ?ys. (LENGTH ys = LENGTH (pat_vars p)) /\
-            (env1 = ZIP (REVERSE (pat_vars p), ys) ++ env)``,
-  STRIP_TAC \\ completeInduct_on `pat_size p` \\ REPEAT STRIP_TAC
-  \\ FULL_SIMP_TAC std_ss [PULL_FORALL]
-  \\ Cases_on `p` \\ FULL_SIMP_TAC (srw_ss()) [pmatch'_def,pat_vars_def,bind_def]
-  THEN1 (Q.EXISTS_TAC `[x2]` \\ EVAL_TAC \\ FULL_SIMP_TAC std_ss [])
-  THEN1 (Cases_on `x2`
-    \\ FULL_SIMP_TAC (srw_ss()) [pmatch'_def,pat_vars_def,bind_def]
-    \\ Cases_on `l = l'` \\ Cases_on `lit_same_type l l'`
-    \\ FULL_SIMP_TAC (srw_ss()) [pmatch'_def,pat_vars_def,bind_def,LENGTH_NIL])
-  \\ POP_ASSUM MP_TAC \\ POP_ASSUM (K ALL_TAC)
-  \\ Cases_on `x2` \\ TRY (Cases_on `o'`) \\ TRY (Cases_on `o''`)
-  \\ FULL_SIMP_TAC (srw_ss()) [pmatch'_def,pat_vars_def,bind_def]
-  \\ SRW_TAC [] [] \\ REPEAT (POP_ASSUM MP_TAC)
-  \\ Q.SPEC_TAC (`l`,`l`) \\ Q.SPEC_TAC (`l'`,`l1`)
-  \\ Q.SPEC_TAC (`env`,`env`) \\ Q.SPEC_TAC (`env1`,`env1`) THEN1
-   (Induct_on `l` \\ Cases_on `l1` \\ FULL_SIMP_TAC std_ss [LENGTH,ADD1]
-    \\ FULL_SIMP_TAC (srw_ss()) [MAP,FLAT,LENGTH,LENGTH_NIL,ZIP,pmatch'_def]
-    \\ STRIP_TAC \\ STRIP_TAC \\ STRIP_TAC
-    \\ Cases_on `pmatch' s h' h env` \\ FULL_SIMP_TAC (srw_ss()) []
-    \\ REPEAT STRIP_TAC
-    \\ FULL_SIMP_TAC std_ss [AND_IMP_INTRO]
-    \\ Q.PAT_ASSUM `!env1 env l1. bbb ==> bbbb` (MP_TAC o Q.SPECL [`env1`,`l'`,`t`])
-    \\ FULL_SIMP_TAC std_ss []
-    THEN (MATCH_MP_TAC IMP_IMP \\ STRIP_TAC THEN1
-       (REPEAT STRIP_TAC \\ FULL_SIMP_TAC std_ss [pat_size_def]
-        \\ Q.PAT_ASSUM `!x.bbb` MATCH_MP_TAC
-        \\ Q.EXISTS_TAC `x2'` \\ FULL_SIMP_TAC std_ss [] \\ DECIDE_TAC)
-      \\ REPEAT STRIP_TAC
-      \\ Q.PAT_ASSUM `!x.bbb` (MP_TAC o Q.SPECL [`h'`,`h`,`env`])
-      \\ FULL_SIMP_TAC (srw_ss()) []
-      \\ MATCH_MP_TAC IMP_IMP \\ STRIP_TAC THEN1
-       (REPEAT STRIP_TAC \\ FULL_SIMP_TAC std_ss [pat_size_def] \\ DECIDE_TAC)
-      \\ REPEAT STRIP_TAC \\ FULL_SIMP_TAC std_ss []
-      \\ Q.EXISTS_TAC `ys ++ ys'`
-      \\ FULL_SIMP_TAC std_ss [LENGTH_APPEND,APPEND_ASSOC,AC ADD_ASSOC ADD_COMM]
-      \\ FULL_SIMP_TAC std_ss [ZIP_APPEND,LENGTH_REVERSE]))
-  THEN1
-   (Cases_on `store_lookup n s` \\ FULL_SIMP_TAC (srw_ss()) []
-    \\ REPEAT STRIP_TAC
-    \\ Q.PAT_ASSUM `!pp. bbb` (MP_TAC o Q.SPECL [`p'`,`x`,`env`])
-    \\ FULL_SIMP_TAC (srw_ss()) []
-    \\ MATCH_MP_TAC IMP_IMP \\ FULL_SIMP_TAC std_ss [pat_vars_def,pat_size_def]
-    \\ DECIDE_TAC)) |> GEN_ALL;
-
-val int_read_exp_IMP = prove(
-  ``!x2. (int_read_exp x2 = SOME (s,r)) ==>
-         ((x2 = Var s) /\ (r = 0)) \/
-         (x2 = (App (Opn Plus) (Var s) ((Lit (IntLit r))))) \/
-         (x2 = (App (Opn Minus) (Var s) ((Lit (IntLit (0-r))))))``,
-  HO_MATCH_MP_TAC (fetch "-" "int_read_exp_ind")
-  \\ FULL_SIMP_TAC (srw_ss()) [int_read_exp_def]
-  \\ REPEAT STRIP_TAC
-  \\ intLib.COOPER_TAC);
-
-val int_cmp_let_thm = prove(
-  ``EVERY (int_cmp_sem x1 T) b /\ evaluate' s0 x1 x2 (s1,Rval (v)) ==>
-    EVERY (int_cmp_sem (bind n v x1) T) (int_cmp_let n x2 b)``,
-  SIMP_TAC std_ss [int_cmp_let_def]
-  \\ Cases_on `int_read_exp x2` \\ FULL_SIMP_TAC (srw_ss()) []
-  \\ Cases_on `x` \\ FULL_SIMP_TAC (srw_ss()) []
-  \\ Induct_on `b` \\ FULL_SIMP_TAC (srw_ss()) [int_cmp_apply_def]
-  \\ Cases \\ FULL_SIMP_TAC (srw_ss()) [int_cmp_apply_def,int_cmp_sem_def]
-  \\ REPEAT STRIP_TAC \\ Cases_on `q = s` \\ FULL_SIMP_TAC std_ss [EVERY_DEF]
-  \\ FULL_SIMP_TAC std_ss [int_cmp_sem_def,bind_def,lookup_def]
-  THEN (IMP_RES_TAC int_read_exp_IMP \\ FULL_SIMP_TAC std_ss []
-    \\ Q.PAT_ASSUM `evaluate' s0 xx yy zz` MP_TAC
-    \\ ASM_SIMP_TAC (srw_ss()) [Once evaluate'_cases]
-    THEN1 (ONCE_REWRITE_TAC [EQ_SYM_EQ] \\ FULL_SIMP_TAC (srw_ss()) [])
-    \\ REPEAT STRIP_TAC \\ IMP_RES_TAC do_app_IMP
-    \\ FULL_SIMP_TAC (srw_ss()) [do_app_def,evaluate_Lit]
-    \\ Q.PAT_ASSUM `evaluate' s0 xx yy zz` MP_TAC
-    \\ Q.PAT_ASSUM `Lit xx = yy` (ASSUME_TAC o GSYM)
-    \\ ASM_SIMP_TAC (srw_ss()) []
-    \\ Q.PAT_ASSUM `evaluate' s0 xx yy zz` MP_TAC
-    \\ ASM_SIMP_TAC (srw_ss()) [Once evaluate'_cases]
-    \\ FULL_SIMP_TAC (srw_ss()) [opn_lookup_def,evaluate_Lit]
-    \\ ASM_SIMP_TAC (srw_ss()) [Once evaluate'_cases]
-    \\ REPEAT STRIP_TAC \\ FULL_SIMP_TAC std_ss []
-    \\ Q.PAT_ASSUM `-r = i2` (ASSUME_TAC o GSYM)
-    \\ FULL_SIMP_TAC (srw_ss()) [evaluate_Lit]));
-
-val decide_guard_IntUnkown = prove(
-  ``!xs. decide_guard IntUnkown xs = NONE``,
-  Induct \\ FULL_SIMP_TAC std_ss [decide_guard_def]);
-
-val store_same_LEMMA = prove(
-  ``(decide_guard (get_fact x2) b = SOME x) /\
-    evaluate' s x1 x2 (s',Rval (Litv (Bool bb))) ==> (s = s')``,
-  Cases_on `x2` \\ FULL_SIMP_TAC (srw_ss()) [get_fact_def,decide_guard_IntUnkown]
-  \\ Cases_on `o'` \\ FULL_SIMP_TAC (srw_ss()) [get_fact_def,decide_guard_IntUnkown]
-  \\ Cases_on `o''` \\ FULL_SIMP_TAC (srw_ss()) [get_fact_def,decide_guard_IntUnkown]
-  \\ Cases_on `e` \\ FULL_SIMP_TAC (srw_ss()) [get_fact_def,decide_guard_IntUnkown]
-  \\ Cases_on `e0` \\ FULL_SIMP_TAC (srw_ss()) [get_fact_def,decide_guard_IntUnkown]
-  \\ TRY (Cases_on `l` \\ FULL_SIMP_TAC (srw_ss()) [get_fact_def,decide_guard_IntUnkown])
-  \\ TRY (Cases_on `l'` \\ FULL_SIMP_TAC (srw_ss()) [get_fact_def,decide_guard_IntUnkown])
-  \\ TRY (Cases_on `l` \\ FULL_SIMP_TAC (srw_ss()) [get_fact_def,decide_guard_IntUnkown])
-  \\ FULL_SIMP_TAC (srw_ss()) [do_app_def, Once evaluate'_cases]
-  \\ FULL_SIMP_TAC (srw_ss()) [do_app_def, Once evaluate'_cases]
-  \\ FULL_SIMP_TAC (srw_ss()) [do_app_def, Once evaluate'_cases]
-  \\ REPEAT STRIP_TAC
-  \\ TRY (Cases_on `v1` \\ FULL_SIMP_TAC (srw_ss()) [])
-  \\ TRY (Cases_on `v2` \\ FULL_SIMP_TAC (srw_ss()) [])
-  \\ TRY (Cases_on `l` \\ FULL_SIMP_TAC (srw_ss()) [])
-  \\ FULL_SIMP_TAC (srw_ss()) []
-  \\ REPEAT (Q.PAT_ASSUM `Lit vv = xx` (ASSUME_TAC o GSYM))
-  \\ FULL_SIMP_TAC std_ss [evaluate_Lit]);
-
-val INT_IF_OPT_LEMMA = prove(
-  ``(!s x1 x2 x3. evaluate' s x1 x2 x3 ==>
-       !b. EVERY (int_cmp_sem x1 T) b /\ isRval (SND x3) ==>
-           evaluate' s x1 (INT_IF_OPT b x2) x3) /\
-    (!s x1 x2 x3. evaluate_list' s x1 x2 x3 ==>
-       !b. EVERY (int_cmp_sem x1 T) b /\ isRval (SND x3) ==>
-           evaluate_list' s x1 (MAP (INT_IF_OPT b) x2) x3) /\
-    (!s x1 x2 x3 x4. evaluate_match' s x1 x2 x3 x4 ==>
-       !b. EVERY (int_cmp_sem x1 T) b /\ isRval (SND x4) ==>
-           evaluate_match' s x1 x2 (MAT_INT_IF_OPT b x3) x4)``,
-  ONCE_REWRITE_TAC [two_assums]
-  \\ HO_MATCH_MP_TAC evaluate'_ind \\ REPEAT STRIP_TAC
-  \\ FULL_SIMP_TAC std_ss [INT_IF_OPT_def,isRval_def]
-  \\ CONV_TAC (DEPTH_CONV ETA_CONV)
-  \\ TRY (RES_TAC \\ ASM_SIMP_TAC (srw_ss()) [Once evaluate'_cases] \\ NO_TAC)
-  THEN1 (RES_TAC \\ ASM_SIMP_TAC (srw_ss()) [Once evaluate'_cases] \\ METIS_TAC [])
-  THEN1 (RES_TAC \\ ASM_SIMP_TAC (srw_ss()) [Once evaluate'_cases] \\ METIS_TAC [])
-  THEN1 (RES_TAC \\ ASM_SIMP_TAC (srw_ss()) [Once evaluate'_cases] \\ METIS_TAC [])
-  THEN1 (RES_TAC \\ ASM_SIMP_TAC (srw_ss()) [Once evaluate'_cases] \\ METIS_TAC [])
-  THEN1 (RES_TAC \\ ASM_SIMP_TAC (srw_ss()) [Once evaluate'_cases] \\ METIS_TAC [])
-  THEN1 (RES_TAC \\ ASM_SIMP_TAC (srw_ss()) [Once evaluate'_cases] \\ METIS_TAC [])
-  THEN1 (RES_TAC \\ ASM_SIMP_TAC (srw_ss()) [Once evaluate'_cases] \\ METIS_TAC [])
-  THEN1 (RES_TAC \\ ASM_SIMP_TAC (srw_ss()) [Once evaluate'_cases] \\ METIS_TAC [])
-  THEN1 (RES_TAC \\ ASM_SIMP_TAC (srw_ss()) [Once evaluate'_cases] \\ METIS_TAC [])
-  THEN1 (ASM_SIMP_TAC (srw_ss()) [Once evaluate'_cases]
-    \\ DISJ1_TAC \\ Q.EXISTS_TAC `v`
-    \\ FULL_SIMP_TAC std_ss [do_log_def]
-    \\ Cases_on `op` \\ FULL_SIMP_TAC (srw_ss()) []
-    \\ Cases_on `v` \\ FULL_SIMP_TAC (srw_ss()) []
-    \\ Cases_on `l` \\ FULL_SIMP_TAC (srw_ss()) []
-    \\ Cases_on `b'` \\ FULL_SIMP_TAC (srw_ss()) [] \\ METIS_TAC [])
-  THEN1 (ASM_SIMP_TAC (srw_ss()) [Once evaluate'_cases]
-    \\ DISJ1_TAC \\ Q.EXISTS_TAC `v`
-    \\ FULL_SIMP_TAC std_ss [do_log_def] \\ METIS_TAC [])
-  THEN1 (ASM_SIMP_TAC (srw_ss()) [Once evaluate'_cases]
-    \\ DISJ2_TAC \\ DISJ1_TAC \\ Q.EXISTS_TAC `v`
-    \\ FULL_SIMP_TAC std_ss [do_log_def] \\ METIS_TAC [])
-  THEN1
-   (Cases_on `decide_guard (get_fact x2) b`
-    \\ FULL_SIMP_TAC (srw_ss()) [] THEN1
-     (FULL_SIMP_TAC std_ss [do_if_def]
-      \\ REPEAT (BasicProvers.FULL_CASE_TAC)
-      \\ FULL_SIMP_TAC (srw_ss()) []
-      \\ RES_TAC \\ ASM_SIMP_TAC (srw_ss()) [Once evaluate'_cases]
-      \\ DISJ1_TAC \\ Q.EXISTS_TAC `v` \\ ASM_SIMP_TAC (srw_ss()) [do_if_def]
-      \\ Q.EXISTS_TAC `s'` \\ FULL_SIMP_TAC std_ss []
-      THEN1 (Q.PAT_ASSUM `!b.bbb` MATCH_MP_TAC
-        \\ FULL_SIMP_TAC std_ss [add_neg_fact_def,EVERY_DEF]
-        \\ MATCH_MP_TAC (get_fact_thm_F |> GEN_ALL)
-        \\ FULL_SIMP_TAC std_ss [] \\ METIS_TAC [])
-      THEN1 (Q.PAT_ASSUM `!b.bbb` MATCH_MP_TAC
-        \\ FULL_SIMP_TAC std_ss [add_pos_fact_def,EVERY_DEF]
-        \\ MATCH_MP_TAC (get_fact_thm_T |> GEN_ALL)
-        \\ FULL_SIMP_TAC std_ss [] \\ METIS_TAC []))
-    \\ IMP_RES_TAC decide_guard_thm
-    \\ FULL_SIMP_TAC std_ss [do_if_def]
-    \\ Cases_on `v = Litv (Bool T)` \\ FULL_SIMP_TAC std_ss []
-    \\ `s' = s` by METIS_TAC [store_same_LEMMA]
-    \\ FULL_SIMP_TAC std_ss []
-    THEN1 (Cases_on `x` \\ FULL_SIMP_TAC (srw_ss()) []
-      \\ IMP_RES_TAC get_fact_thm_T
-      \\ IMP_RES_TAC decide_guard_IMP
-      \\ IMP_RES_TAC int_cmp_sem_NOT)
-    THEN1 (Cases_on `x` \\ FULL_SIMP_TAC (srw_ss()) []
-      \\ IMP_RES_TAC get_fact_thm_F
-      \\ IMP_RES_TAC decide_guard_IMP
-      \\ IMP_RES_TAC int_cmp_sem_negate
-      \\ IMP_RES_TAC int_cmp_sem_NOT))
-  THEN1 (RES_TAC \\ ASM_SIMP_TAC (srw_ss()) [Once evaluate'_cases] \\ METIS_TAC [])
-  THEN1 (RES_TAC \\ ASM_SIMP_TAC (srw_ss()) [Once evaluate'_cases] \\ METIS_TAC [])
-  THEN1 (RES_TAC \\ ASM_SIMP_TAC (srw_ss()) [Once evaluate'_cases] \\ METIS_TAC [])
-  THEN1 (RES_TAC \\ ASM_SIMP_TAC (srw_ss()) [Once evaluate'_cases] \\ METIS_TAC [])
-  THEN1 (RES_TAC \\ ASM_SIMP_TAC (srw_ss()) [Once evaluate'_cases]
-    \\ DISJ1_TAC \\ Q.LIST_EXISTS_TAC [`v`,`s'`] \\ FULL_SIMP_TAC std_ss []
-    \\ Q.PAT_ASSUM `!b.bbb` MATCH_MP_TAC
-    \\ FULL_SIMP_TAC std_ss [EVERY_APPEND]
-    \\ FULL_SIMP_TAC std_ss [EVERY_FILTER,int_cmp_let_thm]
-    \\ IMP_RES_TAC int_cmp_let_thm
-    \\ FULL_SIMP_TAC std_ss []
-    \\ FULL_SIMP_TAC std_ss [EVERY_MEM]
-    \\ REPEAT STRIP_TAC \\ RES_TAC
-    \\ Cases_on `x`
-    \\ FULL_SIMP_TAC std_ss [int_cmp_sem_def,int_cmp_keep_def]
-    \\ Q.EXISTS_TAC `j` \\ FULL_SIMP_TAC std_ss [MEM,lookup_def,bind_def])
-  THEN1 (RES_TAC \\ ASM_SIMP_TAC (srw_ss()) [Once evaluate'_cases] \\ METIS_TAC [])
-  THEN1 (RES_TAC \\ ASM_SIMP_TAC (srw_ss()) [Once evaluate'_cases] \\ METIS_TAC [])
-  THEN1 (RES_TAC \\ ASM_SIMP_TAC (srw_ss()) [Once evaluate'_cases] \\ METIS_TAC [])
-  THEN1 (RES_TAC \\ ASM_SIMP_TAC (srw_ss()) [Once evaluate'_cases] \\ METIS_TAC [])
-  THEN1 (FULL_SIMP_TAC std_ss [MAT_INT_IF_OPT_def,MAP]
-      \\ ASM_SIMP_TAC (srw_ss()) [Once evaluate'_cases]
-      \\ Q.PAT_ASSUM `!x.bbb` MATCH_MP_TAC
-      \\ FULL_SIMP_TAC std_ss [EVERY_FILTER]
-      \\ FULL_SIMP_TAC std_ss [EVERY_MEM]
-      \\ REPEAT STRIP_TAC \\ RES_TAC
-      \\ IMP_RES_TAC pmatch_lemma
-      \\ FULL_SIMP_TAC std_ss []
-      \\ Cases_on `x`
-      \\ FULL_SIMP_TAC std_ss [int_cmp_sem_def,int_cmp_keep_def]
-      \\ Q.EXISTS_TAC `j` \\ FULL_SIMP_TAC std_ss []
-      \\ `~MEM s' (REVERSE (pat_vars p))` by FULL_SIMP_TAC std_ss [MEM_REVERSE]
-      \\ FULL_SIMP_TAC std_ss [lookup_ZIP_APPEND,LENGTH_REVERSE])
-  THEN1
-     (FULL_SIMP_TAC std_ss [MAT_INT_IF_OPT_def,MAP]
-      \\ ASM_SIMP_TAC (srw_ss()) [Once evaluate'_cases] \\ METIS_TAC []));
-
-val INT_IF_OPT_THM =
-  INT_IF_OPT_LEMMA |> CONJUNCT1 |> Q.SPECL [`s`,`env`,`exp`,`t,Rval res`]
-    |> SIMP_RULE std_ss [isRval_def,PULL_FORALL] |> Q.SPEC `[]`
-    |> REWRITE_RULE [EVERY_DEF]
-    |> Q.GEN `res` |> Q.GEN `t` |> Q.GEN `exp` |> Q.GEN `env` |> Q.GEN `s`
-
-*)
-
 (* top-level optimiser *)
 
 val OPTIMISE_def = Define `
   OPTIMISE =
-    BOTTOM_UP_OPT (opt_sub_add o let_id) o
-    (* INT_IF_OPT [] o *)
-    BOTTOM_UP_OPT abs2let`;
+    BOTTOM_UP_OPT (opt_sub_add o let_id) o BOTTOM_UP_OPT abs2let`;
 
 val Eval_OPTIMISE = store_thm("Eval_OPTIMISE",
   ``Eval env exp P ==> Eval env (OPTIMISE exp) P``,
@@ -724,7 +266,6 @@ val Eval_OPTIMISE = store_thm("Eval_OPTIMISE",
   \\ Q.EXISTS_TAC `res` \\ FULL_SIMP_TAC std_ss [OPTIMISE_def]
   \\ MATCH_MP_TAC BOTTOM_UP_OPT_THM
   \\ SIMP_TAC std_ss [opt_sub_add_thm,let_id_thm]
-  (* \\ MATCH_MP_TAC INT_IF_OPT_THM *)
   \\ MATCH_MP_TAC BOTTOM_UP_OPT_THM
   \\ ASM_SIMP_TAC std_ss [abs2let_thm]);
 
